mu types + de bruijn levels -- to test

sort/sort.sig
@@ -6,9 +6,9 @@
   sbool  : sort 
   sci    : Z -> sort
   scb    : bool -> sort
-  spi    : (sort -> sort) -> sort -> sort -> sort
-  slambda: (sort -> sort) -> sort -> sort -> sort
-  ssig   : (sort -> sort) -> sort -> sort -> sort
+  spi    : (sort -> sort) -> sort -> sort
+  slambda: (sort -> sort) -> sort -> sort
+  ssig   : (sort -> sort) -> sort -> sort
   splus  : sort -> sort -> sort
   sminus : sort -> sort -> sort
   sgt    : sort -> sort -> sort
@@ -16,8 +16,10 @@
   sapp   : sort -> sort -> sort
   sstar  : sort
   site   : sort -> sort -> sort -> sort 
-  spair  : (sort -> sort) -> sort -> sort -> sort
-  sextst : sort -> sort -> sort
+  spair  : sort -> sort -> sort
   sneg   : sort -> sort
   sand   : sort -> sort -> sort
   sor    : sort -> sort -> sort
+  sproj1 : sort -> sort
+  sproj2 : sort -> sort
+  smu    : (sort -> sort) -> sort
