sort/sortcheck.v
@@ -13,36 +13,31 @@ Fixpoint lookup (c:  (list (nat*sort))) (m: nat): option sort :=
   end.
 
 Inductive sortCheck: list (fin*sort) -> fin -> sort -> sort -> Prop :=
-  | sc_lambda: forall c x p e t' n m, sortCheck c m p sstar ->
+  | sc_lambda: forall c p e t' n m, sortCheck c m p sstar ->
                                       let t := betan n p in
                                       (* ctx ext *)
                                       sortCheck (cons (pair m t) c) (S m) e t' ->
-                                      sortCheck c m (slambda x p e) (spi x t t') 
-  | sc_app   : forall c e e' x t t' n m, sortCheck c m e (spi x t t') ->
+                                      sortCheck c m (slambda p e) (spi t t') 
+  | sc_app   : forall c e e' t t' n m, sortCheck c m e (spi t t') ->
                                          sortCheck c m e' t ->
                                          let tt := subst_sort (e' .: svar) t' in
                                          let t'' := betan n tt in
                                          sortCheck c m (sapp e e') t''
-  | sc_pi    : forall c x p p' n m, sortCheck c m p sstar ->
+  | sc_pi    : forall c p p' n m, sortCheck c m p sstar ->
                                     let t := betan n p in
                                     (* ctx ext *)
                                     sortCheck (cons (pair m t) c) (S m) p' sstar ->
-                                    sortCheck c m (spi x p p') sstar
-  | sc_pair  : forall c x p e t' n m, sortCheck c m p sstar ->
-                                      let t := betan n p in
-                                      (* ctx ext *)
-                                      sortCheck (cons (pair m t) c) (S m) e t' ->
-                                      sortCheck c m (spair x p e) (ssig x t t') 
-  | sc_exst : forall c e e' x t t' n m, sortCheck c m e (ssig x t t') ->
-                                        sortCheck c m e' t ->
-                                        let tt := subst_sort (e' .: svar) t' in
-                                        let t'' := betan n tt in
-                                        sortCheck c m (sexst e' e) t''
-  | sc_sig   : forall c x p p' n m, sortCheck c m p sstar ->
+                                    sortCheck c m (spi p p') sstar
+  | sc_pair  : forall c e1 p e2 t' n m, sortCheck c m e1 p ->
+                                          let t := betan n p in
+                                          (* ctx ext *)
+                                          sortCheck (cons (pair m t) c) (S m) e2 t' ->
+                                          sortCheck c m (spair e1 e2) (ssig t t')
+  | sc_sig   : forall c p p' n m, sortCheck c m p sstar ->
                                     let t := betan n p in
                                     (* ctx ext *)
                                     sortCheck (cons (pair m t) c) (S m) p' sstar ->
-                                    sortCheck c m (ssig x p p') sstar
+                                    sortCheck c m (ssig p p') sstar
   | sc_star  : forall c m, sortCheck c m sstar sstar
   | sc_var   : forall c s t' m, Some t' = lookup c s ->
                                 sortCheck c m (svar s) t' 
@@ -73,21 +68,36 @@ Inductive sortCheck: list (fin*sort) -> fin -> sort -> sort -> Prop :=
                                  sortCheck c m (sand e1 e2) sbool
   | sc_or    : forall c e1 e2 m, sortCheck c m e1 sbool ->
                                  sortCheck c m e2 sbool ->
-                                 sortCheck c m (sor e1 e2) sbool.
+                                 sortCheck c m (sor e1 e2) sbool
+  | sc_proj1 : forall c e t t' m, sortCheck c m e (ssig t t') ->
+                                  sortCheck c m (sproj1 e) t
+  | sc_proj2 : forall c e t1 t2 n m, sortCheck c m e (ssig t1 t2) ->
+                                     let tt  := subst_sort ((sproj1 e) .: svar) t2 in
+                                     let tt' := betan n tt in
+                                     sortCheck c m (sproj2 e) tt'
+  | sc_mu    : forall c t e t' m, sortCheck (cons (pair m t) c) (S m) e t' ->
+                                  sortCheck c m (smu e) (spi t t').
 
-Example ex1: sortCheck nil 0 (sapp (slambda (svar 0) sint (sapp (slambda (svar 0) sint (sgt (svar 1) (svar 0))) 
-                                                          (sci 110))) 
-                                   (sci 220))
+(* Eval compute in 
+(betan 3
+(sapp (slambda sint (sapp (slambda sint (sgt (svar 1) (svar 0))) 
+                          (sci 110))) 
+      (sci 220))). *)
+
+
+Example ex1: sortCheck nil 0 (sapp (slambda sint (sapp (slambda sint (sgt (svar 1) (svar 0))) 
+                                                       (sci 110))) 
+                             (sci 220))
              sbool.
 Proof. simpl.
        specialize (sc_app nil
-                          (slambda (svar 0) sint (sapp (slambda (svar 0) sint (sgt (svar 1) (svar 0))) (sci 110)))
+                          (slambda sint (sapp (slambda sint (sgt (svar 1) (svar 0))) (sci 110)))
                           (sci 220)
-                          (svar 0) sint sbool 1
+                          sint sbool 1
        ); intro HS. simpl in HS.
        apply HS; clear HS.
        specialize(sc_lambda nil
-                            (svar 0) sint (sapp (slambda (svar 0) sint (sgt (svar 1) (svar 0))) (sci 110))
+                            sint (sapp (slambda sint (sgt (svar 1) (svar 0))) (sci 110))
                             sbool
                             1 0
        ); intro HL. simpl in HL.
@@ -95,14 +105,14 @@ Proof. simpl.
        apply sc_int.
 
        specialize (sc_app (cons (pair 0 sint) nil) 
-                          (slambda (svar 0) sint (sgt (svar 1) (svar 0)))
+                          (slambda sint (sgt (svar 1) (svar 0)))
                           (sci 110)
-                          (svar 0) sint sbool 0
+                           sint sbool 0
        ); intro HS. simpl in HS.
        apply HS; clear HS.
 
        specialize(sc_lambda (cons (pair 0 sint) nil) 
-                            (svar 0) sint (sgt (svar 1) (svar 0))
+                            sint (sgt (svar 1) (svar 0))
                             sbool
                             1 1
        ); intro HL. simpl in HL.
@@ -115,54 +125,42 @@ Proof. simpl.
        apply sc_cint.
 Qed.
 
-Example ex2: sortCheck nil 0
-             (sexst (sci 220) (sexst (sci 110) (spair (svar 0) sint (spair (svar 0) sint (sgt (svar 1) (svar 0)))))) 
-             sbool.
-Proof. specialize(sc_exst nil
-                          (sexst (sci 110) (spair (svar 0) sint (spair (svar 0) sint (sgt (svar 1) (svar 0)))))
-                          (sci 220) (svar 0) sint sbool 1
+Example ex2: sortCheck (cons (pair 5 sint) (cons (pair 6 sint) nil)) 0
+             (spair (svar 5) (spair (svar 6) (sgt (svar 6) (svar 5))))
+             (ssig sint (ssig sint sbool)).
+Proof. specialize(sc_pair (cons (pair 5 sint) (cons (pair 6 sint) nil))
+                          (svar 5) sint 
+                          (spair (svar 6) (sgt (svar 6) (svar 5)))
+                          (ssig sint sbool) 1 0
        ); intro HS. simpl in HS.
        apply HS; clear HS.
-       specialize(sc_exst nil
-                          (spair (svar 0) sint (spair (svar 0) sint (sgt (svar 1) (svar 0))))
-                          (sci 110) (svar 0) sint (ssig (svar 0) sint sbool) 1
+       apply sc_var. simpl. easy.
+       specialize(sc_pair (cons (pair 0 sint) (cons (pair 5 sint) (cons (pair 6 sint) nil)))
+                         (svar 6) sint 
+                         (sgt (svar 6) (svar 5))
+                         sbool 1 1
        ); intro HS. simpl in HS.
        apply HS; clear HS.
-       specialize(sc_pair nil
-                         (svar 0) sint 
-                         (spair (svar 0) sint (sgt (svar 1) (svar 0)))
-                         (ssig (svar 0) sint sbool) 1
-       ); intro HS. simpl in HS.
-       apply HS; clear HS.
-       apply sc_int.
-       specialize(sc_pair (cons (pair 0 sint) nil) 
-                          (svar 0) sint 
-                          (sgt (svar 1) (svar 0))
-                          sbool 1 1
-       ); intro HS. simpl in HS.
-       apply HS; clear HS.
-       apply sc_int.
+       apply sc_var. simpl. easy.
        apply sc_gt.
        apply sc_var. simpl. easy.
        apply sc_var. simpl. easy.
-       apply sc_cint.
-       apply sc_cint.
 Qed.
 
 Example ex3: sortCheck nil 0
-              (sapp (slambda (svar 0) sint (splus (svar 0) (sci 50))) 
-                    (sapp (slambda (svar 0) sint (sminus (svar 0) (sci 18)))  
+              (sapp (slambda sint (splus (svar 0) (sci 50))) 
+                    (sapp (slambda sint (sminus (svar 0) (sci 18)))  
                           (sci 12)
                   )
             ) sint.
 Proof. specialize (sc_app nil
-                          (slambda (svar 0) sint (splus (svar 0) (sci 50)))
-                          (sapp (slambda (svar 0) sint (sminus (svar 0) (sci 18))) (sci 12))
-                          (svar 0) sint sint 1 0
+                          (slambda sint (splus (svar 0) (sci 50)))
+                          (sapp (slambda sint (sminus (svar 0) (sci 18))) (sci 12))
+                          sint sint 1 0
        ); intro HS. simpl in HS.
        apply HS; clear HS.
        specialize(sc_lambda nil
-                            (svar 0) sint
+                            sint
                             (splus (svar 0) (sci 50))
                             sint 1 0
        ); intro HL. simpl in HL.
@@ -172,13 +170,13 @@ Proof. specialize (sc_app nil
        apply sc_var. simpl. easy.
        apply sc_cint.
        specialize (sc_app nil
-                          (slambda (svar 0) sint (sminus (svar 0) (sci 18)))
+                          (slambda sint (sminus (svar 0) (sci 18)))
                           (sci 12)
-                          (svar 0) sint sint 1 0
+                          sint sint 1 0
        ); intro HS. simpl in HS.
        apply HS; clear HS.
        specialize(sc_lambda nil
-                            (svar 0) sint
+                            sint
                             (sminus (svar 0) (sci 18))
                             sint 1 0
        ); intro HL. simpl in HL.
@@ -191,18 +189,18 @@ Proof. specialize (sc_app nil
 Qed.
 
 Example ex4: sortCheck nil 0
-              (sapp (slambda (svar 0) (spi (svar 0) sint sint) (svar 0)) (slambda (svar 0) sint (splus (svar 0) (sci 5))))
-              (spi (svar 0) sint sint).
+              (sapp (slambda (spi sint sint) (svar 0)) (slambda sint (splus (svar 0) (sci 5))))
+              (spi sint sint).
 Proof. specialize (sc_app nil
-                          (slambda (svar 0) (spi (svar 0) sint sint) (svar 0))
-                          (slambda (svar 0) sint (splus (svar 0) (sci 5)))
-                          (svar 0) (spi (svar 0) sint sint) 
-                          (spi (svar 0) sint sint) 1 0
+                          (slambda (spi sint sint) (svar 0))
+                          (slambda sint (splus (svar 0) (sci 5)))
+                          (spi sint sint) 
+                          (spi sint sint) 1 0
        ); intro HS. simpl in HS.
        apply HS; clear HS.
        specialize(sc_lambda nil
-                            (svar 0) (spi (svar 0) sint sint)
-                            (svar 0) (spi (svar 0) sint sint) 1 0
+                            (spi sint sint)
+                            (svar 0) (spi sint sint) 1 0
        ); intro HL. simpl in HL.
        apply HL; clear HL.
        apply sc_pi with (n := 0).
@@ -211,8 +209,8 @@ Proof. specialize (sc_app nil
        apply sc_var. simpl. easy.
 
        specialize(sc_lambda nil
-                            (svar 0) sint
-                             (splus (svar 0) (sci 5)) sint 1 0
+                            sint
+                            (splus (svar 0) (sci 5)) sint 1 0
        ); intro HL. simpl in HL.
        apply HL; clear HL.
        apply sc_int.
